src/hls/Gible.v
@@ -39,8 +39,8 @@ Require Import compcert.common.Smallstep.
 Require Import compcert.lib.Maps.
 Require Import compcert.verilog.Op.
 
-Require Import Predicate.
-Require Import Vericertlib.
+Require Import vericert.hls.Predicate.
+Require Import vericert.common.Vericertlib.
 
 Definition node := positive.
 Definition predicate := positive.
